theories/Spec.v
@@ -21,18 +21,6 @@ Fixpoint zip {A B} (l: list A) (r: list B): list (A * B) :=
  | _, _ => nil
  end.
 
-Fixpoint zip21 {A B C} (l: list (A * B)) (r: list C): list (A * B * C) :=
- match l, r with
- | cons (a, b) l', cons c r' => cons (a, b, c) (zip21 l' r')
- | _, _ => nil
- end.
-
-Fixpoint zip3 {A B C} (l: list A) (m: list B) (r: list C): list (A * B * C) :=
- match l, m, r with
- | cons a l', cons b m', cons c r' => cons (a, b, c) (zip3 l' m' r')
- | _, _, _ => nil
- end.
-
 Fixpoint merge (l r: list nat): list nat :=
   match l, r with
   | cons m l', cons n r' => cons (m + n) (merge l' r')
@@ -71,9 +59,9 @@ Hint Resolve eq_term : ott_coq_equality.
 (* defns dummy *)
 Inductive dum : Prop :=    (* defn dum *).
 
-Definition subst : Set := (list (var * term)).
-
 Definition environment : Set := (list (var * type)).
+
+Definition subst : Set := (list (var * term)).
 
 Definition ts : Set := (list type).
 
@@ -175,6 +163,8 @@ Definition nat : Set := nat.
 Inductive span : Set := 
  | P_with (σ:store) (N:normal).
 
+Definition linear : Set := (list nat).
+
 Inductive context : Set := 
  | E_var (x:var)
  | E_lam (x:var) (t:type) (E:context)
@@ -184,11 +174,7 @@ Inductive context : Set :=
  | E_fanout (E:context) (E':context)
  | E_let (x:var) (y:var) (E:context) (E':context).
 
-Definition ns : Set := (list var).
-
 Definition set : Set := (list span).
-
-Definition linear : Set := (list (var * type * nat)).
 Lemma eq_context: forall (x y : context), {x = y} + {x <> y}.
 Proof.
   decide equality; auto with ott_coq_equality arith.
@@ -227,7 +213,7 @@ end.
 (** definitions *)
 
 (** funs empty *)
-Fixpoint mt (x1:nat) : ns:=
+Fixpoint mt (x1:nat) : linear:=
   match x1 with
   |  0  =>  nil 
   |  (  (S  n )  )  =>  (cons   0     (mt n )  ) 
@@ -236,41 +222,41 @@ end.
 (** definitions *)
 
 (* defns lfind *)
-Inductive lmem : var -> type -> environment -> ns -> Prop :=    (* defn lmem *)
+Inductive lmem : var -> type -> environment -> linear -> Prop :=    (* defn lmem *)
  | lmem_eq : forall (x:var) (t:type) (Γ:environment),
      lmem x t  (cons ( x ,  t )  Γ )   (cons   1     (mt  (  (len Γ )  )  )  ) 
- | lmem_ne : forall (x:var) (t:type) (Γ:environment) (y:var) (t':type) (ns5:ns),
+ | lmem_ne : forall (x:var) (t:type) (Γ:environment) (y:var) (t':type) (Δ:linear),
       ( x  <>  y )  ->
-     lmem x t Γ ns5 ->
-     lmem x t  (cons ( y ,  t' )  Γ )   (cons   0    ns5 ) .
+     lmem x t Γ Δ ->
+     lmem x t  (cons ( y ,  t' )  Γ )   (cons   0    Δ ) .
 (** definitions *)
 
 (* defns judge_context *)
-Inductive JE : environment -> ns -> context -> type -> Prop :=    (* defn E *)
- | JE_var : forall (Γ:environment) (ns5:ns) (x:var) (t:type),
-     lmem x t Γ ns5 ->
-     JE Γ ns5 (E_var x) t
- | JE_lam : forall (Γ:environment) (ns5:ns) (x:var) (t1:type) (E:context) (t2:type),
-     JE  (cons ( x ,  t1 )  Γ )   (cons   1    ns5 )  E t2 ->
-     JE Γ ns5 (E_lam x t1 E) (t_prod t1 t2)
- | JE_app : forall (Γ:environment) (ns5 ns':ns) (E1 E2:context) (t2 t1:type),
-     JE Γ ns5 E1 (t_prod t1 t2) ->
-     JE Γ ns' E2 t1 ->
-     JE Γ  (merge  ns5   ns' )  (E_app E1 E2) t2
+Inductive JE : environment -> linear -> context -> type -> Prop :=    (* defn E *)
+ | JE_var : forall (Γ:environment) (Δ:linear) (x:var) (t:type),
+     lmem x t Γ Δ ->
+     JE Γ Δ (E_var x) t
+ | JE_lam : forall (Γ:environment) (Δ:linear) (x:var) (t1:type) (E:context) (t2:type),
+     JE  (cons ( x ,  t1 )  Γ )   (cons   1    Δ )  E t2 ->
+     JE Γ Δ (E_lam x t1 E) (t_prod t1 t2)
+ | JE_app : forall (Γ:environment) (Δ Δ':linear) (E1 E2:context) (t2 t1:type),
+     JE Γ Δ E1 (t_prod t1 t2) ->
+     JE Γ Δ' E2 t1 ->
+     JE Γ  (merge  Δ   Δ' )  (E_app E1 E2) t2
  | JE_tt : forall (Γ:environment),
      JE Γ  (mt  (  (len Γ )  )  )  E_tt t_unit
- | JE_step : forall (Γ:environment) (ns5 ns':ns) (E1 E2:context) (t:type),
-     JE Γ ns5 E1 t_unit ->
-     JE Γ ns' E2 t ->
-     JE Γ  (merge  ns5   ns' )  (E_step E1 E2) t
- | JE_fanout : forall (Γ:environment) (ns5 ns':ns) (E1 E2:context) (t1 t2:type),
-     JE Γ ns5 E1 t1 ->
-     JE Γ ns' E2 t2 ->
-     JE Γ  (merge  ns5   ns' )  (E_fanout E1 E2) (t_prod t1 t2)
- | JE_let : forall (Γ:environment) (ns5 ns':ns) (x y:var) (E1 E2:context) (t3 t1 t2:type),
-     JE Γ ns5 E1 (t_prod t1 t2) ->
-     JE  (cons ( y ,  t2 )   (cons ( x ,  t1 )  Γ )  )   (cons   1     (cons   1    ns' )  )  E2 t3 ->
-     JE Γ  (merge  ns5   ns' )  (E_let x y E1 E2) t3.
+ | JE_step : forall (Γ:environment) (Δ Δ':linear) (E1 E2:context) (t:type),
+     JE Γ Δ E1 t_unit ->
+     JE Γ Δ' E2 t ->
+     JE Γ  (merge  Δ   Δ' )  (E_step E1 E2) t
+ | JE_fanout : forall (Γ:environment) (Δ Δ':linear) (E1 E2:context) (t1 t2:type),
+     JE Γ Δ E1 t1 ->
+     JE Γ Δ' E2 t2 ->
+     JE Γ  (merge  Δ   Δ' )  (E_fanout E1 E2) (t_prod t1 t2)
+ | JE_let : forall (Γ:environment) (Δ Δ':linear) (x y:var) (E1 E2:context) (t3 t1 t2:type),
+     JE Γ Δ E1 (t_prod t1 t2) ->
+     JE  (cons ( y ,  t2 )   (cons ( x ,  t1 )  Γ )  )   (cons   1     (cons   1    Δ' )  )  E2 t3 ->
+     JE Γ  (merge  Δ   Δ' )  (E_let x y E1 E2) t3.
 (** definitions *)
 
 (* defns sat *)
